* fixed admitted cases in the top simulation lemmas of LAA/LAS and some properties of LASInfo/LAAInfo:
The old version proofs of id_rhs_val were correct, but not sufficient to
LAS. It assumed (vev_defs and substable_value) that 
  in f, if v2/v1 are only defined by cmds (non-phinodes/calls/arguments), 
  then [|v1|]=[|v2|].
However, in LAS, the value stored into the first store can be defined by
phinodes, calls or arguments.

So, we reproved id_rhs_val under a weaker condition:
  in f, if v1 >> v2, v2 is only defined by cmds, then [|v1|]=[|v2|].
In LAS, v2 is defined by load, v1 can be defined by anything, and we
know v1 >> v2.

We should also be able to extend id_rhs_val to allow v2 to be phinodes.
To allow v2 to be calls, we have to know the call does not use any
locations that the instructions between v1 and v2 use. 
It is not useful to allow v2 to be an argument for intraprocedural 
optimizations, since they do not change arguments.

I cannot see how the old id_rhs_val can be used by other SSA-based
optimizations. We can 'roll-back' to that version if necessary.



git-svn-id: https://webdav.seas.upenn.edu/svn/sol/vol@3844 eef5ea85-cc2e-0410-bd84-0fae1f012da8

src3.0/Transforms/id_rhs_val.v
@@ -10,6 +10,7 @@ Require Import trans_tactic.
 
 Definition DGVMap := @Opsem.GVsMap DGVs.
 
+(* go to analysis.v *)
 Definition value_in_scope (v0:value) (ids0:ids) : Prop :=
 match v0 with
 | value_const _ => True
@@ -25,6 +26,7 @@ forall gvs1 gvs2,
   Opsem.getOperandValue TD v2 lc gl = Some gvs2 ->
   gvs1 = gvs2.
 
+(* go to analysis.v *)
 Definition inscope_of_ec (ec:@Opsem.ExecutionContext DGVs) : option ids :=
 let '(Opsem.mkEC f b cs tmn lc als) := ec in
 match cs with
@@ -98,6 +100,7 @@ match c with
 | _ => True (* We may also consider call/excall, but ignore them so far *)
 end.
 
+(* Invariant: in f, v2 >> v1 /\ v1 is defined by c => [|v1|] = [|v2|] *)
 Definition vev_defs (v1 v2:value) F TD M gl (f:fdef) (lc:DGVMap) c ids0: Prop :=
   F = f ->
   (value_in_scope v2 ids0 ->
@@ -110,18 +113,7 @@ Definition vev_defs (v1 v2:value) F TD M gl (f:fdef) (lc:DGVMap) c ids0: Prop :=
            else True
        end
    | _ => True
-   end) /\
-  (value_in_scope v1 ids0 ->
-   match Opsem.getOperandValue TD v1 lc gl with
-   | Some gv1 =>
-       match v2 with
-       | value_const _ => True
-       | value_id id2 =>
-           if (id2 == getCmdLoc c) then eval_rhs TD M gl lc c gv1
-           else True
-       end
-   | _ => True
-  end).
+   end).
 
 Definition vev_ExecutionContext v1 v2 F TD M gl (ec:Opsem.ExecutionContext)
   : Prop :=
@@ -148,7 +140,7 @@ let '(OpsemAux.mkCfg s td _ gl _ ) := cfg in
 let '(Opsem.mkState ecs M) := S in
 vev_ECStack v1 v2 F td M gl ecs.
 
-Definition sustable_cmd (c:cmd) : Prop :=
+Definition substable_cmd (c:cmd) : Prop :=
 match c with
 | insn_call _ _ _ _ _ _ _ => False
 | insn_free _ _ _ => False
@@ -161,13 +153,23 @@ match v with
 | value_const _ => True
 | value_id vid =>
     match lookupInsnViaIDFromFdef f vid with
-    | Some (insn_cmd c) => sustable_cmd c
+    | Some (insn_cmd c) => substable_cmd c
     | _ => False
     end
 end.
 
+(* go to analysis.v 
+   v1 >> v2 == id1 >> id2 \/ v1 is constant
+*)
+Definition valueDominates (f:fdef) (v1 v2:value) : Prop :=
+match v1, v2 with
+| value_id id1, value_id id2 => idDominates f id1 id2
+| value_const _, _ => True
+| _, _ => False
+end.
+
 Definition substable_values TD gl (f:fdef) (v1 v2:value) : Prop :=
-substable_value f v1 /\ substable_value f v2 /\
+substable_value f v1 /\ valueDominates f v2 v1 /\
 match v1, v2 with
 | value_const vc1, value_const vc2 =>
     @Opsem.const2GV DGVs TD gl vc1 = Opsem.const2GV TD gl vc2
@@ -175,7 +177,7 @@ match v1, v2 with
 end.
 
 Lemma eval_rhs_det: forall td M gl lc c gv1 gv2,
-  sustable_cmd c ->
+  substable_cmd c ->
   eval_rhs td M gl lc c gv1 -> eval_rhs td M gl lc c gv2 -> gv1 = gv2.
 Proof.
   destruct c; simpl; intros; destruct_exists; destruct_ands;
@@ -183,9 +185,10 @@ Proof.
 Qed.
 
 Lemma wf_defs_updateAddAL: forall v1 v2 F td Mem gl F' lc' c ids1 ids2 g0
-  (Huniq: uniqFdef F') l1 ps1 cs1 tmn1
+  (Huniq: uniqFdef F') l1 ps1 cs1 tmn1 
   (H : blockInFdefB (block_intro l1 ps1 cs1 tmn1) F' = true)
   (H0 : In c cs1)
+  (Hinscope: ret ids1 = inscope_of_cmd F' (block_intro l1 ps1 cs1 tmn1) c)
   (Hvals : substable_values td gl F v1 v2)
   (Hvinscope2 : vev_defs v1 v2 F td Mem gl F' lc' c ids1)
   (Hinscope2' : wf_defs v1 v2 F td gl F' lc' ids1)
@@ -193,11 +196,12 @@ Lemma wf_defs_updateAddAL: forall v1 v2 F td Mem gl F' lc' c ids1 ids2 g0
   (Heval: eval_rhs td Mem gl lc' c g0),
   wf_defs v1 v2 F td gl F' (updateAddAL _ lc' (getCmdLoc c) g0) ids2.
 Proof.
+Local Opaque inscope_of_cmd.
   intros.
   destruct Heq as [Hinc1 Hinc2].
-  destruct Hvals as [Hval1 [Hval2 _]].
+  destruct Hvals as [Hval1 [Hdom _]].
   intros EQ gvsa gvsb Hina Hinb Hgeta Hgetb; subst.
-  destruct Hvinscope2 as [J1 J2]; auto.
+  unfold vev_defs in Hvinscope2.
   unfold wf_defs in Hinscope2'.
   destruct v1 as [vid1 | vc1]; simpl in *.
   Case "v1 = vid1".
@@ -215,36 +219,33 @@ Proof.
 
         SSSCase "vid2 <> c".
           rewrite <- lookupAL_updateAddAL_neq in Hgetb; auto.
-          rewrite Hgetb in J1.
           assert (In vid2 ids1) as Hin.
             apply Hinc2 in Hinb. simpl in Hinb.
             destruct Hinb; subst; try congruence; auto.
+          apply Hvinscope2 in Hin; auto. rewrite Hgetb in Hin.
           erewrite IngetCmdsIDs__lookupCmdViaIDFromFdef in Hval1; eauto.
           eapply eval_rhs_det; eauto.
 
       SSCase "vid1 <> c".
         rewrite <- lookupAL_updateAddAL_neq in Hgeta; auto.
-        rewrite Hgeta in J2.
         assert (In vid1 ids1) as Hin.
           apply Hinc2 in Hina. simpl in Hina.
           destruct Hina; subst; try congruence; auto.
         destruct (vid2 == getCmdLoc c); subst.
         SSSCase "vid2 == c".
-          rewrite lookupAL_updateAddAL_eq in Hgetb.
-          inv Hgetb.
-          erewrite IngetCmdsIDs__lookupCmdViaIDFromFdef in Hval2; eauto.
-          eapply eval_rhs_det; eauto.
+	  admit. (* vid1 in ids1 ==> vid1 >> c
+                    vid2 == c ==> vid1 >> vid2!! *)
 
         SSSCase "vid2 <> c".
           rewrite <- lookupAL_updateAddAL_neq in Hgetb; auto.
-          rewrite Hgetb in J1.
+          rewrite Hgetb in Hvinscope2.
           assert (In vid2 ids1) as Hin'.
             apply Hinc2 in Hinb. simpl in Hinb.
             destruct Hinb; subst; try congruence; auto.
           eauto.
 
     SCase "v2 = vc2".
-      rewrite Hgetb in J1.
+      rewrite Hgetb in Hvinscope2.
       destruct (vid1 == getCmdLoc c); subst.
       SSCase "vid1 == c".
         rewrite lookupAL_updateAddAL_eq in Hgeta.
@@ -260,22 +261,10 @@ Proof.
         eapply Hinscope2'; eauto.
 
   Case "v1 = vc1".
-    rewrite Hgeta in J2.
     destruct v2 as [vid2 | vc2]; simpl in *; eauto.
     SCase "v2 = vid1".
-      destruct (vid2 == getCmdLoc c); subst.
-      SSCase "vid2 == c".
-        rewrite lookupAL_updateAddAL_eq in Hgetb.
-        inv Hgetb.
-        erewrite IngetCmdsIDs__lookupCmdViaIDFromFdef in Hval2; eauto.
-        eapply eval_rhs_det; eauto.
-
-      SSCase "vid2 <> c".
-        rewrite <- lookupAL_updateAddAL_neq in Hgetb; auto.
-        assert (In vid2 ids1) as Hin.
-          apply Hinc2 in Hinb. simpl in Hinb.
-          destruct Hinb; subst; try congruence; auto.
-        eapply Hinscope2'; eauto.
+      tauto.
+Transparent inscope_of_cmd.
 Qed.
 
 Lemma wf_defs_eq : forall ids2 ids1 v1 v2 F td gl F' lc',
@@ -461,7 +450,7 @@ Lemma wf_defs_br_aux : forall v1 v2 F0 TD gl S M lc l' ps' cs' lc' F tmn' b
   (Hinc : incl (ListSet.set_diff eq_atom_dec ids0' (getPhiNodesIDs ps')) t),
   wf_defs v1 v2 F0 TD gl F lc' ids0'.
 Proof.
-  intros. destruct Hvals as [Hval1 [Hval2 _]].
+  intros. destruct Hvals as [Hval1 [Hdom _]].
   unfold Opsem.switchToNewBasicBlock in Hswitch. simpl in Hswitch.
   intros EQ gvs1 gvs2 Hin1 Hin2 Hget1 Hget2; subst.
   remember (Opsem.getIncomingValuesForBlockFromPHINodes TD ps' b gl lc) as R1.
@@ -481,7 +470,10 @@ Proof.
     destruct v2 as [vid2 | vc2]; simpl in *; eauto.
     SCase "v2 = vid2".
       assert (~ In vid2 (getPhiNodesIDs ps')) as Hnotin2.
-        eapply substable_value_isnt_phi; eauto.
+        admit. (* vid1 in ids0' /\ vid1 notin ps' /\ vid2 in ps' ==>  
+                    v1d1 >> vid2 !!
+                  But, we should extend idDominates to allow PHI to prove this!
+               *)
       assert (Hnotin2' := Hnotin2).
       apply ListSet.set_diff_intro with (x:=ids0')(Aeq_dec:=eq_atom_dec)
         in Hnotin2; auto.
@@ -493,15 +485,7 @@ Proof.
   Case "v1 = vc1".
     destruct v2 as [vid2 | vc2]; simpl in *; eauto.
     SCase "v2 = vid2".
-      assert (~ In vid2 (getPhiNodesIDs ps')) as Hnotin.
-        eapply substable_value_isnt_phi; eauto.
-      assert (Hnotin' := Hnotin).
-      apply ListSet.set_diff_intro with (x:=ids0')(Aeq_dec:=eq_atom_dec)
-        in Hnotin; auto.
-      apply Hinc in Hnotin. assert (HeqR1':=HeqR1).
-      eapply OpsemProps.getIncomingValuesForBlockFromPHINodes_spec8 in HeqR1;
-        eauto.
-      eapply OpsemProps.updateValuesForNewBlock_spec7 in Hget2; eauto.
+      tauto.
 Qed.
 
 Lemma inscope_of_tmn_br_aux : forall S M F l3 ps cs tmn ids0 l' ps' cs' tmn'
@@ -865,17 +849,14 @@ Lemma preservation_dbCall_case : forall fid fa rt la va lb td lc gl
   wf_defs v1 v2 F td gl
     (fdef_intro (fheader_intro fa rt fid la va) lb) lc (getArgsIDs la).
 Proof.
-  intros. destruct Hvals as [Hval1 [Hval2 Hcst]].
+  intros. destruct Hvals as [Hval1 [Hdom Hcst]].
   assert (incl nil (bound_blocks lb)) as J.
     intros x J. inv J.
   intros EQ gvs1 gvs2 Hin1 Hin2 Hget1 Hget2; subst.
   destruct v1 as [vid1 | vc1].
     eapply substable_value_isnt_arg in Hval1; eauto.
     simpl in Hin1. congruence.
-  destruct v2 as [vid2 | vc2].
-    eapply substable_value_isnt_arg in Hval2; eauto.
-    simpl in Hin2. congruence.
-
+  destruct v2 as [vid2 | vc2]; try tauto.
     simpl in *. rewrite Hget1 in Hcst. rewrite Hget2 in Hcst. congruence.
 Qed.
 
@@ -1165,6 +1146,7 @@ Require Import program_sim.
 
 Lemma initLocals__id_rhs_val_wf_defs : forall pinfo fid l' fa rt la va
   lb gvs lc CurLayouts CurNamedts initGlobal v1 v2 (Hwfpi: WF_PhiInfo pinfo)
+  (Hdom: valueDominates (PI_f pinfo) v2 v1)
   (Huniq: uniqFdef (fdef_intro (fheader_intro fa rt fid la va) lb))
   (Hinit : Opsem.initLocals
      (OpsemAux.initTargetData CurLayouts CurNamedts Mem.empty)
@@ -1186,15 +1168,14 @@ Proof.
     intros x J. inv J.
   apply fold_left__bound_blocks with (fh:=fheader_intro fa rt fid la va)(l0:=l')
     (init:=getArgsIDs la) in J.
-  destruct J as [r J]. unfold l in *.
-  rewrite J.
+  destruct J as [r J]. unfold l in *. simpl in *. uniq_result.
   intros EQ gvs1 gvs2 Hinscope1 Hinscope2 Hget1 Hget2.
-  clear - Huniq EQ Hget1 Hinit.
-  admit. (* lid cannot be in lc, << *)
+  admit. (* in la, there are no domination relations. *)
 Qed.
 
 Lemma s_genInitState__id_rhs_val: forall S main VarArgs cfg IS pinfo v1 v2
   (HwfS : wf_system S) (Hwfpi: WF_PhiInfo pinfo) 
+  (Hdom: valueDominates (PI_f pinfo) v2 v1)
   (Hinit : @Opsem.s_genInitState DGVs S main VarArgs Mem.empty = ret (cfg, IS)),
   wf_State v1 v2 (PI_f pinfo) cfg IS.
 Proof.
